saving example TAL code

TAL.v
@@ -5,19 +5,6 @@ Require Import Bool Arith Vector Maps.
 (* 10 registers *)
 Definition K := 10.
 Definition registers := total_map nat.
-
-(*
-Check lt_0_Sn.
-Check lt_n_Sn.
-Check lt_n_S 1 7 (lt_n_S 0 6 (lt_0_Sn 5)).
-
-Fixpoint prf_of_lt_n_m (n m : nat) : (n < m) :=
-  match n , m with
-  | S n', S m' => lt_n_S n' m' (prf_of_lt_n_m n' m')
-  | 0 , S m' => lt_0_Sn m'
-  | _,_ => 
-  end.
-*)
       
 Inductive aexp : Type :=
 | ANum : nat -> aexp
@@ -27,13 +14,13 @@ Inductive aexp : Type :=
 
 Inductive instr : Type :=
 | IAss : forall d : nat, (d < K) -> aexp -> instr
-| IAdd : forall d s : nat, (d < K) /\ (s < K) -> instr
-| ISub : forall d s : nat, (d < K) /\ (s < K) -> instr
+| IAdd : forall d s : nat, (d < K) -> (s < K) -> instr
+| ISub : forall d s : nat, (d < K) -> (s < K) -> instr
 | IIf : forall d : nat, (d < K) -> aexp -> instr
 | ISeq : instr -> instr -> instr
 | IJmp : aexp -> instr.               
 
-Definition heaps := total_map instr.
+Definition heaps := partial_map instr.
 
 (* Machine State *)
 Inductive st : Type :=
@@ -49,12 +36,29 @@ Fixpoint aeval (a : aexp) (R : registers) : nat :=
   end.
 
 Inductive ieval : instr -> st -> st -> Prop :=
-| R_IAss : forall H R I d a1 pf, ieval (IAss d pf a1) (St H R I) (St H (t_update R (Id d) (aeval a1 R)) I)
-| R_IAdd : forall H R I d s pf, ieval (IAdd d s pf) (St H R I) (St H (t_update R (Id s) (aeval (AReg d) R + aeval (AReg s) R)) I)
-| R_ISub : forall H R I d s pf, ieval (IAdd d s pf) (St H R I) (St H (t_update R (Id s) (aeval (AReg d) R - aeval (AReg s) R)) I)
-| R_IJmp : forall H R I I' v, H (Id (R (Id v))) = I' -> ieval (IJmp (AReg v)) (St H R I) (St H R I')                            
-| R_IIf_EQ : forall H R I I' v r pf, aeval (AReg r) R = 0 -> (H (Id (R (Id v)))) = I' -> ieval (IIf r pf (AReg v)) (St H R I) (St H R I')
-| R_IIf_NEQ : forall H R I I' v r pf, aeval (AReg r) R <> 0 -> (H (Id (R (Id v)))) = I' -> ieval (IIf r pf (AReg v)) (St H R I) (St H R I)   
+| R_IAss : forall H R I d a1 pf, ieval (IAss d pf a1) (St H R (ISeq (IAss d pf a1) I)) (St H (t_update R (Id d) (aeval a1 R)) I)
+| R_IAdd : forall H R I d s pf1 pf2, ieval (IAdd d s pf1 pf2) (St H R (ISeq (IAdd d s pf1 pf2) I)) (St H (t_update R (Id s) (aeval (AReg d) R + aeval (AReg s) R)) I)
+| R_ISub : forall H R I d s pf1 pf2, ieval (ISub d s pf1 pf2) (St H R (ISeq (ISub d s pf1 pf2) I)) (St H (t_update R (Id s) (aeval (AReg d) R - aeval (ANum s) R)) I)
+| R_IJmp_Succ : forall H R I I' v, H (Id (R (Id v))) = Some I' -> ieval (IJmp (AReg v)) (St H R I) (St H R I')
+| R_IJmp_Fail : forall H R I v, H (Id (R (Id v))) = None -> ieval I (St H R I) (St H R I)
+| R_IIf_EQ : forall H R I I' v r pf, aeval (AReg r) R = 0 -> (H (Id (R (Id v)))) = Some I' -> ieval (IIf r pf (AReg v)) (St H R I) (St H R I')
+| R_IIf_NEQ : forall H R I v r pf, aeval (AReg r) R <> 0 -> ieval (IIf r pf (AReg v)) (St H R (ISeq (IIf r pf (AReg v)) I)) (St H R I)   
 | R_ISeq : forall st st' st'' i1 i2, ieval i1 st st' -> ieval i2 st' st'' -> ieval (ISeq i1 i2) st st''
+| R_IStuck : forall st i, ieval i st st
 .
 
+Definition empty_heap : heaps := empty.
+
+Definition empty_regs : registers := t_empty 0.
+
+Definition threeLEten := (lt_n_S 2 9 (lt_n_S 1 8 (lt_n_S 0 7 (lt_0_Sn 6)))).
+Definition twoLEten :=  (lt_n_S 1 9 (lt_n_S 0 8 (lt_0_Sn 7))).
+Definition oneLEten :=  (lt_n_S 0 9 (lt_0_Sn 8)).
+
+
+
+Definition init_heap := (update (update (update empty_heap (Id 1) (ISeq (IAss 3 threeLEten (ANum 0)) (IJmp (ANum 2)))) (Id 2) (ISeq (IIf 1 oneLEten (ANum 3)) (ISeq (IAdd 2 3 twoLEten threeLEten) (ISeq (ISub 1 1 oneLEten oneLEten) (IJmp (ANum 2))) ))  )  (Id 3) (IJmp (AReg 4)) ).
+
+Print init_heap.
+
+Example ieval_example1 : ieval (IAss 3 threeLEten (ANum 0)) (St init_heap empty_regs I) .
